thys/MFODL_Monitor_Devel/Monitor_Impl.thy
@@ -726,12 +726,12 @@ lemma [code]:
   by(auto simp: upd_nested_max_tstp_def split:option.splits prod.splits)
 
 lemma [code]:
-  "add_new_mmauaux args rel1 rel2 nt (mmuaux, aggaux, done_agg) =
+  "add_new_mmauaux args rel1 rel2 nt (mmuaux, aggaux) =
     (case args_agg args of 
      None \<Rightarrow> let (tp, tss, tables, len, maskL, maskR, a1_map, a2_map, tstp_map, done, done_length) = add_new_mmuaux args rel1 rel2 nt mmuaux in
-  ((tp, tss, tables, len, maskL, maskR, a1_map, a2_map, tstp_map, done, done_length), aggaux, replicate done_length None) |
+  ((tp, tss, tables, len, maskL, maskR, a1_map, a2_map, tstp_map, done, done_length), aggaux) |
      Some aggargs \<Rightarrow>
-    (let ((tp, tss, tables, len, maskL, maskR, a1_map, a2_map, tstp_map, done, done_length), aggaux, done_agg) = shift_mmauaux args nt (mmuaux, aggaux, done_agg);
+    (let ((tp, tss, tables, len, maskL, maskR, a1_map, a2_map, tstp_map, done, done_length), aggaux) = shift_mmauaux args nt (mmuaux, aggaux);
     I = args_ivl args; pos = args_pos args;
     new_tstp = (if memL I 0 then Inr tp else Inl nt);
     tstp_map = Mapping.update tp nt tstp_map;
@@ -750,7 +750,7 @@ lemma [code]:
     to_add = to_add_set (tp - len) m tmp;
     aggaux = insert_maggaux' aggargs to_add aggaux;
     tss = append_queue nt tss in
-    ((tp + 1, tss, tables, len + 1, maskL, maskR, a1_map, a2_map', tstp_map, done, done_length), aggaux, done_agg)))"
+    ((tp + 1, tss, tables, len + 1, maskL, maskR, a1_map, a2_map', tstp_map, done, done_length), aggaux)))"
   by(auto simp del: add_new_mmuaux.simps simp add: to_add_set_def  upd_nested_max_tstp_def split:option.splits prod.splits)
 
 (*<*)
